\section{First Examples}

\subsection{The Simplest Examples}
% end

\subsection{Linear Systems with Constant Coefficients}
  \paragraph{2.}
  \begin{solution}
    $\,$ \\
    (a) $x_i(t)=k_i e^t$ where $i=1,2,3$. \\
    (b) $x_1(t)=k_1e^t$, $x_2(t)=k_2e^{-2t}$ and $x_3(t)=k_3$. \\
    (b) $x_1(t)=k_1e^t$, $x_2(t)=k_2e^{-2t}$ and $x_3(t)=k_3e^{2t}$.
  \end{solution}

  \paragraph{4.}
  \begin{solution}
    \[
      x\hp(t) = 
      \begin{bmatrix}
        e^t \\ 4e^{2t} \\ 8e^{2t}  
      \end{bmatrix} =
      \begin{bmatrix}
        1 &   & \\
          & 2 & \\
          &   & 2 
      \end{bmatrix}
      \begin{bmatrix}
        e^t \\ 2e^{2t} \\ 4e^{2t}  
      \end{bmatrix} =
      \begin{bmatrix}
        1 &   &   \\
          & 2 &   \\
          & 2 & 1 
      \end{bmatrix}
      \begin{bmatrix}
        e^t \\ 2e^{2t} \\ 4e^{2t}  
      \end{bmatrix}.
    \]
  \end{solution}

  \paragraph{6.}
  \begin{solution}
    Suppose that $A=\diag(a_1,\dots,a_n)$, then $x_i(t)=K_i\exp(a_it)$. Hence,
    $x(t)\to 0$ as $t\to\infty$ for all solutions iff $a_i<0$ for each $i=1, 2, 
    \dots,n$.
  \end{solution}

  \paragraph{8.}
  \begin{proof}
    $\,$ \\
    (a) It follows immediately that both the differential operator and $A$ are
    linear operators. \\
    (b) Since every solution is of form $x(t)=(K_1e^t, K_2e^{-2t})$, $u(t)=(e^t,
    0)$ and $v(t)=(0, e^{-2t})$ are two suitable solutions.
  \end{proof}
% end
